freeze

Curve25519Dalek/Specs/Backend/Serial/U64/Field/FieldElement51/Mul.lean
@@ -17,6 +17,18 @@ Source: curve25519-dalek/src/backend/serial/u64/field.rs -/
 open Aeneas.Std Result
 namespace curve25519_dalek.backend.serial.u64.field.FieldElement51.Mul
 
+-- duplicated?
+@[progress]
+theorem m_spec (x y : U64) :
+    ∃ result, mul.m x y = ok (result) ∧
+    result.val = x.val * y.val := by
+  unfold mul.m
+  progress*
+  -- BEGIN TASK
+  simp [*]
+  scalar_tac
+  -- END TASK
+
 /-
 natural language description:
 
@@ -28,7 +40,7 @@ natural language specs:
     • The function always succeeds (no panic)
     • Field51_as_Nat(result) ≡ Field51_as_Nat(lhs) * Field51_as_Nat(rhs) (mod p)
 -/
-
+set_option maxHeartbeats 1000000 in
 /-- **Spec and proof concerning `backend.serial.u64.field.FieldElement51.Mul.mul`**:
 - No panic (always returns successfully)
 - The result, when converted to a natural number, is congruent to the product of the inputs modulo p
@@ -41,6 +53,80 @@ theorem mul_spec (lhs rhs : Array U64 5#usize)
     ∃ r, mul lhs rhs = ok r ∧
     Field51_as_Nat r ≡ (Field51_as_Nat lhs) * (Field51_as_Nat rhs) [MOD p] ∧
     (∀ i < 5, r[i]!.val < 2 ^ 52) := by
-  sorry
+  unfold mul
+  have := hrhs 0 (by simp);
+  have := hrhs 1 (by simp);
+  have := hrhs 2 (by simp);
+  have := hrhs 3 (by simp);
+  have := hrhs 4 (by simp);
+  have := hlhs 0 (by simp);
+  have := hlhs 1 (by simp);
+  have := hlhs 2 (by simp);
+  have := hlhs 3 (by simp);
+  have := hlhs 4 (by simp);
+  progress; progress; progress; progress;
+  progress; progress; progress; progress;
+  progress; progress; progress; progress;
+  progress; progress
+  · /-have : (lhs.val)[0]!.val * (rhs.val)[0]!.val ≤ (2 ^ 54 - 1) * (2 ^ 54 - 1) := by
+        scalar_tac +nonLin
+    have : (lhs.val)[4]!.val * (rhs).val[1]!.val ≤ (2 ^ 54 - 1) * (2 ^ 54 - 1) := by
+        scalar_tac +nonLin
+    --simp [*]
+    -/
+    simp only [*]
+    ring_nf
+    scalar_tac
+    --ring_nf
+
+  progress; progress; progress
+  · simp only [*]
+    ring_nf
+    scalar_tac
+  progress; progress; progress
+  · simp only [*]
+    ring_nf
+    scalar_tac
+  progress; progress; progress
+  · sorry
+  progress; progress; progress
+  · sorry
+  progress; progress
+  · sorry
+  progress; progress
+  · sorry
+  progress; progress
+  · sorry
+
+set_option maxHeartbeats 10000000 in
+@[progress]
+theorem mul_spec' (lhs rhs : Array U64 5#usize)
+    (hlhs : ∀ i < 5, lhs[i]!.val < 2 ^ 54) (hrhs : ∀ i < 5, rhs[i]!.val < 2 ^ 54) :
+    ∃ r, mul lhs rhs = ok r ∧
+    Field51_as_Nat r ≡ (Field51_as_Nat lhs) * (Field51_as_Nat rhs) [MOD p] ∧
+    (∀ i < 5, r[i]!.val < 2 ^ 52) := by
+  unfold mul
+  have := hrhs 0 (by simp);
+  have := hrhs 1 (by simp);
+  have := hrhs 2 (by simp);
+  have := hrhs 3 (by simp);
+  have := hrhs 4 (by simp);
+  have := hlhs 0 (by simp);
+  have := hlhs 1 (by simp);
+  have := hlhs 2 (by simp);
+  have := hlhs 3 (by simp);
+  have := hlhs 4 (by simp);
+  progress* by (simp only [*]; ring_nf; scalar_tac) -- this may work, but it's way too slow
+
 
 end curve25519_dalek.backend.serial.u64.field.FieldElement51.Mul
+
+def inBounds (a : Array U64 5#usize) := ∀ i < 5, a[i]!.val < 2 ^ 54
+
+@[scalar_tac]
+theorem inBounds_imp {a} (h0 : inBounds a) i (h : i < 5) :
+    a[i]!.val < 2 ^ 54 := by sorry
+
+example a (h0 : inBounds a) i (h : i < 5) :
+    a[i]!.val < 2 ^ 54 := by
+    scalar_tac
